src/program_proof/buf/buf_proof.v
@@ -1460,7 +1460,7 @@ Proof.
   wp_call.
   iDestruct (is_slice_small_sz with "Hsrc") as %Hsrc_sz.
   iDestruct (is_slice_small_sz with "Hdst") as %Hdst_sz.
-  wp_apply (wp_SliceTake byteT); first by word.
+  wp_apply wp_SliceTake; first by word.
   wp_pures.
   wp_apply wp_SliceSkip'; first by (iPureIntro; word).
   iDestruct (slice_small_split _ (word.divu dstoff 8) with "Hdst")
